RedScoping.v
@@ -1,0 +1,24 @@
+Require Import Prelude.
+Require Import Expr Scoping Reduction.
+Notation ren_scop xi i j := (forall v, v < i -> xi v < j).
+
+Lemma All_sub D : forall sigma C e, (All D C e).[sigma] = All D C.[up sigma] e.[sigma].
+Proof. induction D; intros; simpl; rewrite asms; autosubst. Qed.
+
+Hint Resolve All_sub.
+Hint Rewrite All_sub.
+Hint Rewrite All_sub : autosubst.
+
+Lemma closed_step e e' n : e ::> e' -> closed_at n e -> closed_at n e'.
+Proof. move=> He'; move: n; induction He'; simpl in *; intros; subst;
+  autounfold in *; destr bands;
+  try solve[repeat (apply andb_true_intro; split); auto|apply cons_id_scoped || apply cons2_id_scoped; firstorder].  
+  - apply closed_lift with (i := 0); try eapply Reduction.const_vals_closed; eassumption || auto.
+  - apply cons2_id_scoped; auto.
+    apply rall_scoped; simpl; auto; autorewrite with core.
+    apply sub_vars_scoped with (i := (2 + n)); auto.
+    intros; change (ren (iterate upren 2 (+1)) v) with (Bind (upnren 2 (+1) v)); simpl; auto.
+    pose proof (ren_upnren 2 n n.+1 (+1)); firstorder.
+Qed.
+
+Hint Resolve closed_step.
