Scoping.v
@@ -8,15 +8,15 @@ Proof.
   destruct e; 
   repeat match goal with
            | [i : var |- _] => exact: (i < l)
-           | [e : {bind exp} |- _] => apply (closed_at l.+1) in e; apply (&& e)
-           | [e : exp |- _] => apply (closed_at l) in e; apply (&& e)
+           | [e : {bind ?n of exp} |- _] => apply (&& closed_at (n + l) e); clear e
+           | [e : exp |- _] => apply (&& closed_at l e); clear e
            | _ => exact: true
          end.
 Defined.
 
 (* While we're at it *)
 Ltac mk_size T f :=
-  repeat match goal with [e : T |- _] => apply f in e; apply (+ e) | _ => exact: 1 end.
+  simpl in *; repeat match goal with [e : T |- _] => apply f in e; apply (+ e) | _ => exact: 1 end.
       
 Fixpoint term_size (e : exp) : nat.
   destruct e; mk_size exp term_size.
@@ -26,7 +26,14 @@ Notation closed := (closed_at 0).
 
 Notation closed_sub l sigma := (forall i, i < l -> sigma i = Bind i).
 Lemma closed_up : forall l sigma, closed_sub l sigma -> closed_sub l.+1 (up sigma).
-  intros. destruct i; asimpl; eauto. rewrite H; eauto. Qed.
+Proof. intros. destruct i; asimpl; eauto. rewrite H; eauto. Qed.
+Hint Resolve closed_up.
+Lemma closed_upn : forall n l sigma, closed_sub l sigma -> closed_sub (n + l) (upn n sigma).
+Proof. induction n; intros; asimpl; auto.
+  replace (upn n.+1 sigma i) with (up (upn n sigma) i) by autosubst.
+  destruct i; asimpl; erewrite ?IHn; try eassumption; auto.
+Qed.
+Hint Resolve closed_upn.
 
 Tactic Notation "destr" "bands" := 
   repeat match goal with
@@ -34,13 +41,18 @@ Tactic Notation "destr" "bands" :=
            | [H: _ && _ = true |- _] => apply andb_prop in H; destruct H
          end.
 
+Hint Rewrite Bool.orb_false_r Bool.orb_true_iff.
+Hint Rewrite Bool.andb_negb_r Bool.andb_true_iff.
+Hint Resolve andb_prop Bool.orb_prop.
+
 (* This proof is gross for stupid reasons - fix later *)
 Hint Resolve andb_true_intro.
 Lemma closed_lift : forall e i j, i <= j -> closed_at i e -> closed_at j e.
+Proof.
   induction e; intros; simpl in *; try reflexivity; unfold is_true in *;
   apply leq_trans with (n := i) ||
     (destr bands;
-    repeat match goal with [H : forall i j : nat, _ |- _] => extend (H i j); extend (H i.+1 j.+1) end);
+    repeat match goal with [H : forall i j : nat, _ |- _] => extend (H i j); extend (H i.+1 j.+1); extend (H i.+2 j.+2) end);
     auto 10.
 Qed.
 
@@ -50,17 +62,17 @@ Qed.
 Lemma closed_under : forall i j sigma, i <= j -> closed_sub j sigma -> closed_sub i sigma.
 Proof. induction i; intros; try solve by inversion. apply H0. eapply leq_trans; eauto. Qed.
 
-Hint Resolve closed_up.
 Lemma closed_at_sub_id : forall e i sigma, closed_sub i sigma -> closed_at i e -> e.[sigma] = e.
-  induction e; intros i sigma Hsig; extend (closed_up _ _ Hsig); 
-  intros; simpl in *; unfold is_true in *;
-  repeat match goal with [H : _ && _ = true |- _] => apply andb_prop in H; destr_ands end;
-  f_equal; eauto.
+Proof. 
+  induction e; intros i sigma Hsig; (* ; pose proof (closed_up _ _ Hsig); pose proof (closed_up _ _ (closed_up _ _ Hsig)); *)
+  intros; simpl in *; auto;
+  autounfold in *; autorewrite with core in *; destr_logic; f_equal; eauto.
 Qed.
 
-Hint Rewrite closed_at_sub_id using assumption.
+Hint Rewrite closed_at_sub_id using assumption || now auto.
 
 Lemma sub_0 : forall sigma, closed_sub 0 sigma. intros; solve by inversion. Qed.
+Hint Resolve sub_0.
 
 Notation sub_vars i j sigma := (forall v, v < i -> closed_at j (sigma v)).
 
@@ -86,18 +98,22 @@ Lemma upnren_mono_less : forall n v sigma, mono sigma -> upnren n sigma v <= sig
 Proof. induction n; intros; rewrite ?iterate_S; auto. transitivity (upnren n sigma v); auto. Qed.
 Hint Resolve upnren_mono_less.
 
-Hint Rewrite Bool.orb_false_r Bool.orb_true_iff.
-Hint Rewrite Bool.andb_negb_r Bool.andb_true_iff.
-Hint Resolve andb_prop Bool.orb_prop.
-
-Hint Rewrite up_upren_n_internal up_upren_internal using auto.
+Hint Rewrite up_upren_n_internal up_upren_internal using now auto.
 Hint Resolve up_upren_n_internal up_upren_internal.
 Hint Resolve andb_true_intro.
 
 Notation sub_eq sigma tau := (forall v, sigma v = tau v).
 Lemma up_resp_eq : forall sigma tau, sub_eq sigma tau -> sub_eq (up sigma) (up tau). destruct v; asimpl; f_equal; auto. Qed.
 Hint Resolve up_resp_eq.
+Lemma upn_resp_eq n : forall sigma tau, sub_eq sigma tau -> sub_eq (upn n sigma) (upn n tau). 
+Proof. induction n; intros; auto.
+  repeat match goal with [|-context[upn ?n.+1 ?sigma ?v]] => change (upn n.+1 sigma v) with (up (upn n sigma) v) end.
+  apply up_resp_eq; auto.
+Qed.
+Hint Resolve upn_resp_eq.
 Lemma sub_vars_tms : forall e sigma tau, sub_eq sigma tau -> e.[sigma] = e.[tau]. induction e; intros; simpl; f_equal; auto. Qed.
+Hint Resolve sub_vars_tms.
+Hint Rewrite sub_vars_tms using assumption || now auto.
 Canonical sub_eq_refl : reflexive (var -> exp) (fun sigma tau => sub_eq sigma tau). constructor. Qed.
 
 Hint Rewrite sub_vars_tms using auto.
@@ -108,13 +124,29 @@ Lemma ren_upren : forall i j xi, closed_ren i j xi -> closed_ren i.+1 j.+1 (upre
 Proof. destruct v; simpl; intros; firstorder. Qed.
 Hint Resolve ren_upren.
 
+Lemma ren_upnren n : forall i j xi, closed_ren i j xi -> closed_ren (n + i) (n + j) (upnren n xi).
+Proof. induction n; intros; rewrite ?iterate_0 ?iterate_S; auto.
+  apply ren_upren with (i := n + i); firstorder.
+Qed.
+Hint Resolve ren_upnren.  
+
+SearchRewrite (up (ren _)).
+SearchRewrite (upn _ (ren _)).
+
 Lemma ren_closed_corr e : forall i j xi, closed_ren i j xi -> closed_at i e -> closed_at j e.[ren xi].
 Proof. induction e; simpl; intros; autounfold in *; destr bands;
+  repeat match goal with [|-context[?t.[upn ?v (ren ?xi)]]] => replace t.[upn v (ren xi)] with t.[ren (upnren v xi)] 
+                           by (autorewrite with core; reflexivity) end;
   try solve[auto|   (* this would just be eauto, but it seems to be broken with closed_at *)
+            repeat (apply andb_true_intro; split);
+            eapply IHe || eapply IHe0 || eapply IHe1 || eapply IHe2;
+            eassumption || apply ren_upnren || apply ren_upren; now auto|
+            (* basically the same, but asimpl's first *)
             asimpl; repeat (apply andb_true_intro; split);
             eapply IHe || eapply IHe0 || eapply IHe1 || eapply IHe2;
-            eassumption || apply ren_upren; auto].
+            eassumption || apply ren_upnren || apply ren_upren; now auto].
 Qed.
+
 Hint Resolve ren_closed_corr.
 
 Lemma ren_wk_scoped : forall i j, closed_ren i (j + i) (+j). auto. Qed.
@@ -148,9 +180,17 @@ Hint Resolve wk1_scoped.
 Lemma up_vars : forall i j sigma, sub_vars i j sigma -> sub_vars i.+1 j.+1 (up sigma).
 Proof. intros. destruct v; asimpl; auto. Qed.
 
+Hint Resolve up_vars.
+
 Lemma wk_vars : forall i, sub_vars i i.+1 (wk 1). auto. Qed.
 
-Hint Resolve up_vars wk_vars.
+Lemma upn_vars n : forall i j sigma, sub_vars i j sigma -> sub_vars (n + i) (n + j) (upn n sigma).
+Proof. induction n; auto. destruct v; simpl; intros; auto.
+  asimpl; apply wk1_scoped; eapply IHn; eassumption.
+Qed.
+
+Hint Resolve up_vars upn_vars wk_vars.
+
 Tactic Notation "htry" :=
   repeat match goal with
              [H: ?P -> _, H2 : ?P |- _] => extend (H H2)
@@ -162,7 +202,8 @@ Lemma sub_vars_scoped : forall e i j sigma, sub_vars i j sigma -> closed_at i e 
 Proof. move=>e i j sigma Hs He.
   move: i He j sigma Hs.
   induction e; intros; simpl; rewrite asms; auto;
-  simpl in *; unfold is_true in *; destr bands; try apply up_vars; eassumption || auto.
+  try (apply upn_vars || apply up_vars);
+  solve [simpl in *; unfold is_true in *; destr bands; eassumption || auto].
 Qed.
 
 Hint Resolve sub_vars_scoped.
@@ -172,6 +213,7 @@ Proof. intros; apply closed_at_sub_id with (i := 0); intros; solve by inversion 
 
 Lemma cons_vars_scoped e sigma i j : sub_vars i j sigma -> closed_at j e -> sub_vars i.+1 j (e .: sigma). intros; destruct v; simpl; auto. Qed.
 Hint Resolve cons_vars_scoped.
+
 Lemma cons_scoped sigma i j v e : sub_vars i j sigma -> closed_at j v -> closed_at i.+1 e -> closed_at j e.[v .: sigma].
 Proof. intros; eapply sub_vars_scoped; eassumption || apply cons_vars_scoped; auto. Qed.
 Hint Resolve cons_scoped.
@@ -180,6 +222,10 @@ Lemma cons_id_scoped i v e : closed_at i v -> closed_at i.+1 e -> closed_at i e.
 Proof. apply cons_scoped with (i := i); auto. Qed.
 Hint Resolve cons_id_scoped.
 
+Lemma cons2_id_scoped i v1 v2 e : closed_at i v1 -> closed_at i v2 -> closed_at i.+2 e -> closed_at i e.[v1,v2/]. 
+Proof. intros; apply cons_scoped with (i := i.+1); auto.
+  intros; change ((v2 .: ids) v) with (Bind v).[v2/]; auto.
+Qed.
 (* Axiom consts_wf : forall nm t, const_tys nm = Some t -> closed t. *)
 (* Axiom conv_sub : forall sigma t t', conv t t' -> conv t.[sigma] t'.[sigma]. *)
 
